isabelle/Chapter18_1_Language.thy
@@ -22,32 +22,16 @@ where "insert n (Var v) = Var (incr n v)"
     | "insert n (Appl e1 e2) = Appl (insert n e1) (insert n e2)"
     | "insert n (Fix e) = Fix (insert (next n) e)"
 
-primrec remove :: "var => expr => expr"
-where "remove n (Var v) = Var (subr n v)"
-    | "remove n (Num x) = Num x"
-    | "remove n Zero = Zero"
-    | "remove n (Succ e) = Succ (remove n e)"
-    | "remove n (IsZ et e0 es) = IsZ (remove n et) (remove n e0) (remove (next n) es)"
-    | "remove n (Lam e) = Lam (remove (next n) e)"
-    | "remove n (Appl e1 e2) = Appl (remove n e1) (remove n e2)"
-    | "remove n (Fix e) = Fix (remove (next n) e)"
-
-primrec subst' :: "var => expr => expr => expr"
-where "subst' n e' (Var v) = (if v = n then e' else Var v)"
-    | "subst' n e' (Num x) = Num x"
-    | "subst' n e' Zero = Zero"
-    | "subst' n e' (Succ e) = Succ (subst' n e' e)"
-    | "subst' n e' (IsZ et e0 es) = 
-                      IsZ (subst' n e' et) (subst' n e' e0) (subst' (next n) (insert first e') es)"
-    | "subst' n e' (Lam e) = Lam (subst' (next n) (insert first e') e)"
-    | "subst' n e' (Appl e1 e2) = Appl (subst' n e' e1) (subst' n e' e2)"
-    | "subst' n e' (Fix e) = Fix (subst' (next n) (insert first e') e)"
-
-definition subst :: "expr => var => expr => expr"
-where "subst e' n e = remove first (subst' first (insert first e') e)"
-
-lemma [simp]: "remove n (insert n e) = e"
-by (induction e arbitrary: n, simp_all)
+primrec subst :: "expr => var => expr => expr"
+where "subst e' n (Var v) = (if v = n then e' else Var (subr n v))"
+    | "subst e' n (Num x) = Num x"
+    | "subst e' n Zero = Zero"
+    | "subst e' n (Succ e) = Succ (subst e' n e)"
+    | "subst e' n (IsZ et e0 es) = 
+                      IsZ (subst e' n et) (subst e' n e0) (subst (insert first e') (next n) es)"
+    | "subst e' n (Lam e) = Lam (subst (insert first e') (next n) e)"
+    | "subst e' n (Appl e1 e2) = Appl (subst e' n e1) (subst e' n e2)"
+    | "subst e' n (Fix e) = Fix (subst (insert first e') (next n) e)"
 
 lemma [simp]: "canswap m n ==> insert m (insert n e) = insert (next n) (insert m e)"
 by (induction e arbitrary: n m, simp_all)
